ver3_less_complex/common/sets.dfy
@@ -4,25 +4,6 @@ module M_Set {
 
     import opened Std.Collections.Set
 
-    method SetToSeq<T>(s: set<T>) returns (sq: seq<T>)
-    ensures |sq| == |s| // The length of the sequence equals the size of the set
-    ensures forall i :: 0 <= i < |sq| ==> sq[i] in s // All elements in the sequence are from the set
-    ensures forall i, j :: 0 <= i < j < |sq| ==> sq[i] != sq[j] // The sequence has no duplicates
-    {
-        sq := [];
-        var remaining := s;
-        while |remaining| > 0
-            invariant |sq| + |remaining| == |s|
-            invariant forall x :: x in sq ==> x in s
-            invariant forall x :: x in sq ==> x !in remaining
-            invariant forall i, j :: 0 <= i < j < |sq| ==> sq[i] != sq[j]
-        {
-            var x :| x in remaining;
-            sq := sq + [x];
-            remaining := remaining - {x};
-        }
-    }
-
     lemma LemmaProperSubsetCardinality<T>(x: set<T>, y:set<T>)
     requires x < y
     ensures |x| < |y|
@@ -102,4 +83,25 @@ module M_Set {
     {
         Set.LemmaSubsetSize(x, y);
     }
+
+    ghost predicate isTotoalOrder<T(!new)> (R : (T, T) -> bool)
+    {
+        && (forall x :: R(x, x))
+        && (forall x, y :: R(x, y) && R(y, x) ==> x == y)
+        && (forall x, y, z :: R(x, y) && R(y, z) ==> R(x, z))
+        && (forall x, y :: R(x, y) || R(y, x))
+    }
+
+    // function setToSeq<T(!new)> (s : set<T>, R : (T, T) -> bool) : (r : seq<T>)
+    // requires isTotoalOrder(R)
+    // ensures forall i | 0 <= i < |r| :: r[i] in s
+    // ensures forall e | e in s :: e in r
+    // {
+    //     if s == {} then []
+    //     else
+
+    // }
+
+
+
 }
